%% skrive det om så du bruker det som et teorem.

KKT-conditions are first order necessary conditions for a solution in nonlinear programming to be optimal. It is therefore of great importance that these conditions are fulfilled.
%We adapt the notation $x = (x_1,\cdots x_n, y_1,\cdots,y_n)$.\\
Assume $x^*$ is a optimal point, then the KKT-conditions, for a  minimization problem with only equality constraints are:
\begin{itemize}
\item $\mathcal{L}(x^*,\lambda^*) = E(x^*)- \sum\limits_{i=1}^{n+1}\lambda_i c_i(x^*)$
\item $\nabla_x \mathcal{L}(x^*,\lambda^*) = 0$
\item $c_i(x^*) = 0$
\end{itemize}

For our problem this becomes: \\
$\mathcal{L}(x^*,\lambda^*) = \sum \limits_{i=1}^{n+1} m_ig\frac{y_i+y_{i-1}}{2} -\sum\limits_{i=1}^{n+1}\lambda_i [(x_i-x_{i-1})^2 + (y_i-y_{i-1})^2-l^2_i]$\\
The KKT-conditions for our problem is then
\begin{itemize}
\item $\nabla_{x_i}\mathcal{L}(x^*,\lambda^*)= -2 \lambda_i (x_i-x_{i-1}) +2 \lambda_{i+1}(x_{i+1}-x_{i})=0$\\
\item $\nabla_{y_i}\mathcal{L}(x^*,\lambda^*)= m_i g - 2 \lambda_i (y_i-y_{i-1}) +2 \lambda_{i+1}(y_{i+1}-y_{i})=0$\\
\item $c_i(x) = (x_i-x_{i-1})^2 + (y_i-y_{i-1})^2-l^2_i=0$\\
\end{itemize}

%!!!!!!!!!!!!!!!!!!!!Må ta med dette for kantene også?!!!!!!!!!!!!!!!!!!!!!!
Assuming that the boundarys are known, we only have $n$ unknowns $ i \in { 1,\cdots, n}.$\\
